More support for weak head reduction, including a simpset for rewriting with it.

examples/lambda/barendregt/head_reductionScript.sml
@@ -1,8 +1,11 @@
 open HolKernel Parse boolLib bossLib
 
 open chap3Theory pred_setTheory termTheory boolSimps
+open binderLib
 
 val _ = new_theory "head_reduction"
+
+fun Store_thm(trip as (n,t,tac)) = store_thm trip before export_rewrites [n]
 
 val _ = set_trace "Unicode" 1
 
@@ -20,7 +23,7 @@ val _ = overload_on ("-h->*", ``hreduce1^*``)
 
 val hreduce_ccbeta = store_thm(
   "hreduce_ccbeta",
-  ``∀M N. M -h-> N ⇒ compat_closure beta M N``,
+  ``∀M N. M -h-> N ⇒ M -β-> N``,
   HO_MATCH_MP_TAC hreduce1_ind THEN SRW_TAC [][cc_beta_thm] THEN
   METIS_TAC []);
 
@@ -81,7 +84,7 @@ val hreduce1_rwts = store_thm(
   ]);
 
 val hnf_def = Define`hnf M = ∀N. ¬(M -h-> N)`;
-val hnf_thm = store_thm(
+val hnf_thm = Store_thm(
   "hnf_thm",
   ``(hnf (VAR s) ⇔ T) ∧
     (hnf (M @@ N) ⇔ hnf M ∧ ¬is_abs M) ∧
@@ -90,13 +93,11 @@ val hnf_thm = store_thm(
   Cases_on `is_abs M` THEN SRW_TAC [][hreduce1_rwts] THEN
   Q.SPEC_THEN `M` FULL_STRUCT_CASES_TAC term_CASES THEN
   FULL_SIMP_TAC (srw_ss()) [hreduce1_rwts]);
-val _ = export_rewrites ["hnf_thm"]
 
-val hnf_tpm = store_thm(
+val hnf_tpm = Store_thm(
   "hnf_tpm",
   ``∀M π. hnf (π·M) = hnf M``,
   HO_MATCH_MP_TAC simple_induction THEN SRW_TAC [][]);
-val _ = export_rewrites ["hnf_tpm"]
 
 val hreduce1_unique = store_thm(
   "hreduce1_unique",
@@ -147,6 +148,134 @@ val wh_head = store_thm(
 val _ = set_fixity "-w->*" (Infix(NONASSOC, 450))
 val _ = overload_on ("-w->*", ``RTC (-w->)``)
 
+val _ = reveal "Y"
+val whY1 = store_thm(
+  "whY1",
+  ``Y @@ f -w-> Yf f``,
+  SRW_TAC [][chap2Theory.Y_def, chap2Theory.Yf_def, LET_THM,
+             Once weak_head_cases] THEN
+  NEW_ELIM_TAC THEN REPEAT STRIP_TAC THEN DISJ1_TAC THEN
+  SRW_TAC [DNF_ss][LAM_eq_thm] THEN DISJ1_TAC THEN
+  SRW_TAC [][chap2Theory.SUB_LAM_RWT, LET_THM] THEN NEW_ELIM_TAC THEN
+  SRW_TAC [][LAM_eq_thm, tpm_fresh]);
+
+val whY2 = store_thm(
+  "whY2",
+  ``Yf f -w-> f @@ Yf f``,
+  SRW_TAC [][chap2Theory.Yf_def, LET_THM, Once weak_head_cases] THEN
+  NEW_ELIM_TAC THEN SRW_TAC [DNF_ss][LAM_eq_thm, lemma14b]);
+
+val wh_unique = store_thm(
+  "wh_unique",
+  ``M -w-> N₁ ∧ M -w-> N₂ ⇒ (N₁ = N₂)``,
+  METIS_TAC [hreduce1_unique, wh_head]);
+
+val whnf_def = Define`
+  whnf M = ∀N. ¬(M -w-> N)
+`;
+
+val hnf_whnf = store_thm(
+  "hnf_whnf",
+  ``hnf M ⇒ whnf M``,
+  METIS_TAC [hnf_def, whnf_def, wh_head]);
+
+val bnf_hnf = store_thm(
+  "bnf_hnf",
+  ``bnf M ⇒ hnf M``,
+  METIS_TAC [hnf_def, beta_normal_form_bnf, corollary3_2_1, hreduce_ccbeta]);
+
+val bnf_whnf = store_thm(
+  "bnf_whnf",
+  ``bnf M ⇒ whnf M``,
+  METIS_TAC [hnf_whnf, bnf_hnf]);
+
+val whnf_thm = Store_thm(
+  "whnf_thm",
+  ``whnf (VAR s) ∧
+    (whnf (M @@ N) ⇔ ¬is_abs M ∧ whnf M) ∧
+    whnf (LAM v M)``,
+  REPEAT CONJ_TAC THEN SRW_TAC [][whnf_def, Once weak_head_cases] THEN
+  EQ_TAC THEN SRW_TAC [][FORALL_AND_THM] THENL [
+    Q.SPEC_THEN `M` FULL_STRUCT_CASES_TAC term_CASES THEN SRW_TAC [][] THEN
+    METIS_TAC [],
+    Q.SPEC_THEN `M` FULL_STRUCT_CASES_TAC term_CASES THEN
+    FULL_SIMP_TAC (srw_ss()) []
+  ]);
+
+val wh_weaken_cong = store_thm(
+  "wh_weaken_cong",
+  ``whnf N ⇒ M₁ -w->* M₂ ⇒ (M₁ -w->* N = M₂ -w->* N)``,
+  SIMP_TAC (srw_ss()) [EQ_IMP_THM, IMP_CONJ_THM] THEN CONJ_TAC THENL [
+    Q_TAC SUFF_TAC `∀M N. M -w->* N ⇒ ∀N'. M -w->* N' ∧ whnf N' ⇒ N -w->* N'`
+          THEN1 METIS_TAC [] THEN
+    HO_MATCH_MP_TAC relationTheory.RTC_INDUCT THEN SRW_TAC [][] THEN
+    METIS_TAC [relationTheory.RTC_CASES1, whnf_def, wh_unique],
+
+    METIS_TAC [relationTheory.RTC_CASES_RTC_TWICE]
+  ]);
+
+val wh_app_congL = store_thm(
+  "wh_app_congL",
+  ``M -w->* M' ==> M @@ N -w->* M' @@ N``,
+  STRIP_TAC THEN Q.ID_SPEC_TAC `N` THEN POP_ASSUM MP_TAC THEN
+  MAP_EVERY Q.ID_SPEC_TAC [`M'`, `M`] THEN
+  HO_MATCH_MP_TAC relationTheory.RTC_INDUCT THEN SRW_TAC [][] THEN
+  METIS_TAC [relationTheory.RTC_RULES, weak_head_rules]);
+
+val tpm_whead_I = store_thm(
+  "tpm_whead_I",
+  ``∀M N. M -w-> N ⇒ π·M -w-> π·N``,
+  HO_MATCH_MP_TAC weak_head_ind THEN SRW_TAC [][weak_head_rules, tpm_subst]);
+
+val whead_gen_bvc_ind = store_thm(
+  "whead_gen_bvc_ind",
+  ``∀P f. (∀x. FINITE (f x)) ∧
+          (∀v M N x. v ∉ f x ⇒ P (LAM v M @@ N) ([N/v]M) x) ∧
+          (∀M₁ M₂ N x. (∀z. P M₁ M₂ z) ⇒ P (M₁ @@ N) (M₂ @@ N) x)
+        ⇒
+          ∀M N. M -w-> N ⇒ ∀x. P M N x``,
+  REPEAT GEN_TAC THEN STRIP_TAC THEN
+  Q_TAC SUFF_TAC `∀M N. M -w-> N ⇒ ∀π x. P (π·M) (π·N) x`
+        THEN1 METIS_TAC [tpm_NIL] THEN
+  HO_MATCH_MP_TAC weak_head_ind THEN SRW_TAC [][tpm_subst] THEN
+  Q_TAC (NEW_TAC "z") `{lswapstr π v} ∪ FV (π·M) ∪ FV (π·N) ∪ f x` THEN
+  `LAM (lswapstr π v) (π·M) = LAM z ([VAR z/lswapstr π v](π·M))`
+     by SRW_TAC [][SIMPLE_ALPHA] THEN
+  `[π·N/lswapstr π v](π·M) = [π·N/z] ([VAR z/lswapstr π v](π·M))`
+     by SRW_TAC [][lemma15a] THEN
+  SRW_TAC [][]);
+
+val whead_bvcX_ind = save_thm(
+  "whead_bvcX_ind",
+  whead_gen_bvc_ind |> Q.SPECL [`λM N x. P' M N`, `λx. X`]
+                    |> SIMP_RULE (srw_ss()) []
+                    |> Q.INST [`P'` |-> `P`]
+                    |> Q.GEN `X` |> Q.GEN `P`);
+
+val wh_substitutive = store_thm(
+  "wh_substitutive",
+  ``∀M N. M -w-> N ⇒ [P/v]M -w-> [P/v]N``,
+  HO_MATCH_MP_TAC whead_bvcX_ind THEN Q.EXISTS_TAC `FV P ∪ {v}` THEN
+  SRW_TAC [][weak_head_rules] THEN
+  Q.MATCH_ABBREV_TAC `LAM z ([P/v]M) @@ [P/v]N -w-> [P/v] ([N/z]M)` THEN
+  METIS_TAC [chap2Theory.substitution_lemma, weak_head_rules]);
+
+val whstar_substitutive = store_thm(
+  "whstar_substitutive",
+  ``∀M N. M -w->* N ⇒ [P/v]M -w->* [P/v]N``,
+  HO_MATCH_MP_TAC relationTheory.RTC_INDUCT THEN SRW_TAC [][] THEN
+  METIS_TAC [relationTheory.RTC_RULES, wh_substitutive]);
+
+val whstar_betastar = store_thm(
+  "whstar_betastar",
+  ``∀M N. M -w->* N ⇒ M -β->* N``,
+  HO_MATCH_MP_TAC relationTheory.RTC_INDUCT THEN SRW_TAC [][] THEN
+  METIS_TAC [relationTheory.RTC_RULES, wh_head, hreduce_ccbeta]);
+
+val whstar_lameq = store_thm(
+  "whstar_lameq",
+  ``M -w->* N ⇒ M == N``,
+  METIS_TAC [betastar_lameq, whstar_betastar]);
 
 val _ = set_trace "Unicode" 0
 
